src/program_proof/lockservice/fmcounter_map.v
@@ -2,7 +2,7 @@ From iris.algebra Require Import gmap lib.mono_nat.
 From iris.proofmode Require Import base tactics classes.
 From Perennial.base_logic Require Import lib.own.
 From iris.bi.lib Require Import fractional.
-From Perennial.program_proof Require Import disk_prelude.
+From Perennial.program_proof Require Import proof_prelude.
 
 Class fmcounter_mapG Σ :=
    { fmcounter_map_inG :> inG Σ (gmapUR u64 mono_natR) }.
