src/program_proof/memkv/memkv_clerk_proof.v
@@ -1,8 +1,7 @@
 From Perennial.program_proof Require Import disk_prelude.
 From Goose.github_com.mit_pdos.gokv Require Import memkv.
-From Perennial.goose_lang Require Import ffi.grove_ffi.
 From Perennial.program_proof.lockservice Require Import rpc.
-From Perennial.program_proof.memkv Require Export common_proof memkv_coord_clerk_proof memkv_shard_clerk_proof.
+From Perennial.program_proof.memkv Require Export rpc_axioms common_proof memkv_coord_clerk_proof memkv_shard_clerk_proof.
 
 Section memkv_clerk_proof.
 
