src/program_proof/memkv/rpc_axioms.v
@@ -1,0 +1,81 @@
+From Perennial.program_proof Require Import dist_prelude.
+From Goose.github_com.mit_pdos.gokv.urpc Require Import rpc.
+From Perennial.goose_lang.lib Require Import slice.typed_slice.
+
+Section rpc_axioms.
+Context `{!heapG Σ}.
+
+Axiom handler_is : ∀ (X:Type) (host:u64) (rpcid:u64) (Pre:X → list u8 → iProp Σ)
+                     (Post:X → list u8 → list u8 → iProp Σ), iProp Σ.
+
+Axiom handler_is_pers : ∀ X host rpcid pre post, Persistent (handler_is X host rpcid pre post).
+
+Global Instance handler_is_pers_instance X host rpcid pre post : Persistent (handler_is X host rpcid pre post).
+apply handler_is_pers.
+Defined.
+
+Axiom RPCClient_own : ∀ (cl_ptr:loc) (host:u64), iProp Σ.
+
+Axiom wp_MakeRPCClient : ∀ (host:u64) ,
+  {{{
+       True
+  }}}
+    MakeRPCClient #host
+  {{{
+       (cl_ptr:loc), RET #cl_ptr; RPCClient_own cl_ptr host
+  }}}.
+
+Axiom wp_RPCClient__Call : ∀ {X:Type} (x:X) (cl_ptr:loc) (rpcid:u64) (host:u64) req rep_ptr dummy_sl_val (reqData:list u8) Pre Post k,
+  {{{
+      is_slice req byteT 1 reqData ∗
+      rep_ptr ↦[slice.T byteT] dummy_sl_val ∗
+      handler_is X host rpcid Pre Post ∗
+      RPCClient_own cl_ptr host ∗
+      □(▷ Pre x reqData)
+  }}}
+    RPCClient__Call #cl_ptr #rpcid (slice_val req) #rep_ptr @ k ; ⊤
+  {{{
+       (b:bool) rep_sl (repData:list u8), RET #b;
+       rep_ptr ↦[slice.T byteT] (slice_val rep_sl) ∗
+       RPCClient_own cl_ptr host ∗
+       typed_slice.is_slice req byteT 1 reqData ∗
+       typed_slice.is_slice rep_sl byteT 1 repData ∗
+       (⌜b = true⌝ ∨ ⌜b = false⌝ ∗ (▷ Post x reqData repData))
+  }}}.
+
+Definition is_rpcHandler {X:Type} (f:val) Pre Post : iProp Σ :=
+  ∀ (x:X) req rep dummy_rep_sl (reqData:list u8),
+  {{{
+      is_slice req byteT 1 reqData ∗
+      rep ↦[slice.T byteT] (slice_val dummy_rep_sl) ∗
+      ▷ Pre x reqData
+  }}}
+    f (slice_val req) #rep
+  {{{
+       rep_sl (repData:list u8), RET #(); rep ↦[slice.T byteT] (slice_val rep_sl) ∗
+         is_slice rep_sl byteT 1 repData ∗
+         ▷ Post x reqData repData
+  }}}.
+
+Axiom own_RPCServer : loc → gmap u64 val → iProp Σ.
+
+Axiom wp_MakeRPCServer : ∀ (handlers : gmap u64 val) (mref:loc) (def : val) k,
+  {{{
+       map.is_map mref (handlers, def)
+  }}}
+    MakeRPCServer #mref @ k ; ⊤
+  {{{
+      (s:loc), RET #s; own_RPCServer s handlers
+  }}}.
+
+Axiom wp_StartRPCServer : ∀ host (handlers : gmap u64 val) (s : loc) (def : val) k,
+  {{{
+       own_RPCServer s handlers ∗
+      [∗ map] rpcid ↦ handler ∈ handlers, (∃ X Pre Post, handler_is X host rpcid Pre Post ∗ is_rpcHandler handler Pre Post)
+  }}}
+    RPCServer__Serve #s #host @ k ; ⊤
+  {{{
+      RET #(); True
+  }}}.
+
+End rpc_axioms.
